\documentclass{ctexart}
% Required package
\usepackage[UTF8]{ctex}
\usepackage{amsmath,amssymb,amsfonts}
\usepackage{bm}
\usepackage[dvipsnames]{xcolor}

\begin{document}
\fontsize{25.0pt}{\baselineskip}\selectfont

\fontsize{20.0pt}{\baselineskip}\selectfont
\begin{align*}
a_n =\frac{sinx}{1^2} + \frac{sin2x}{2^2} + \cdots + \frac{sinnx}{n^2},\mbox{证明}\{a_n\}\mbox{收敛}
\end{align*}

\pagenumbering{arabic}
\newpage
\pagenumbering{arabic}
\fontsize{16.0pt}{\baselineskip}\selectfont


\begin{align*}
&a_{n+p} - a_n = \frac{sin(n+1)x}{(n+1)^2} + \frac{sin(n+2)x}{(n+2)^2} + \cdots + \frac{sin(n+p)x}{(n+p)^2}\\
&|a_{n+p} - a_n| \le |\frac{sin(n+1)x}{(n+1)^2}| + |\frac{sin(n+2)x}{(n+2)^2}| + \cdots + |\frac{sin(n+p)x}{(n+p)^2}|\\
&\quad\quad\le|\frac{1}{(n+1)^2}| + |\frac{1}{(n+2)^2}| + \cdots + |\frac{1}{(n+p)^2}|\\
&\quad\quad\le|\frac{1}{(n+1)(n)}| + |\frac{1}{(n+2)(n+1)}| + \cdots + |\frac{1}{(n+p)(n+p-1))}|\\
&\quad\quad\le(\frac{1}{n-1} - \frac{1}{n}) + (\frac{1}{n}-\frac{1}{n+1}) + \cdots + (\frac{1}{n+p-1} - \frac{1}{n+p})\\
&\quad\quad=\frac{1}{n-1} - \frac{1}{n+p}\\
&\quad\quad\le\frac{1}{n-1}\\
&\forall \epsilon > 0,\frac{1}{n-1} < \epsilon,\mbox{取N}=【\frac{1}{\epsilon}】+ 1\\
&\forall p \in \mathbb{N}, n>N, |a_{n+p} - a_n| < \epsilon\\
&\mbox{根据柯西收敛定理，得证}&
\end{align*}

\end{document}