\documentclass{ctexart}
% Required package
\usepackage[UTF8]{ctex}
\usepackage{amsmath,amssymb,amsfonts}
\usepackage{bm}

\author{yuanxijie@gmail.com}

\begin{document}


\fontsize{60.0pt}{\baselineskip}\selectfont
$$
\lim_{n\to\infty}{\frac{\sqrt[n]{n!}}{n}} = \frac{1}{e}
$$


\pagenumbering{arabic}

\newpage
\pagenumbering{arabic}
\fontsize{16.0pt}{\baselineskip}\selectfont

$$ \mbox{两边取 ln， 仅需证明} \frac{\ln 1+\ln 2+\cdots+\ln n}{n} - \ln{n} = -1 $$
$$\frac{\ln 1+\ln 2+\cdots+\ln n}{n} - \ln{n} = \frac{\sum\limits_{i=1}^{n}{\ln{i}}-n\ln{n}}{n}$$
$$\makebox[5em][r]{利用 stolz 定律，仅需证明} $$
$$\sum\limits_{i=1}^{n+1}{\ln{i}}-(n+1)\ln{(n+1)} - (\sum\limits_{i=1}^{n}{\ln{i}}-n\ln{n}) = -1\mbox{即可}$$

\begin{align*}
    &\sum\limits_{i=1}^{n+1}{\ln{i}}-(n+1)\ln{n+1} - (\sum\limits_{i=1}^{n}{\ln{i}}-n\ln{n})\\
    &=\ln{(n+1)} - (n+1)\ln{(n+1)} + n\ln(n) \\
    &= n\ln(n) - n\ln{(n+1)}\\
    &= \ln\frac{1}{(1+\frac{1}{n})^n}\\
    e &= \lim_{n\to\infty}(1+\frac{1}{n})^n\\
\end{align*}
得证
\end{document}