\documentclass{ctexart}
% Required package
\usepackage[UTF8]{ctex}
\usepackage{amsmath,amssymb,amsfonts}
\usepackage{bm}
\usepackage[dvipsnames]{xcolor}

\begin{document}
\fontsize{25.0pt}{\baselineskip}\selectfont

$$\mbox{设}f_1(x)=af(x)+bg(x), g_1(x)=cf(x)+dg(x)$$
$$\mbox{且} ad-bc\ne0$$
$$\\$$
$$\quad\quad\mbox{证明：} (f(x), g(x)) = (f_1(x), g_1(x))$$  

\pagenumbering{arabic}
\newpage
\pagenumbering{arabic}
\fontsize{16.0pt}{\baselineskip}\selectfont

\begin{align*}
&\mbox{设}u(x) = (f(x), g(x)), v(x) = (f_1(x), g_1(x))\\
&u(x) | f(x), u(x) | g(x) \Longrightarrow u(x)|af(x) + bg(x),u(x) | cf(x) + dg(x)\\
&\mbox{即}ux(x) | f_1(x) , u(x) | g_1(x) \Longrightarrow u(x) | (f_1(x), g_1(x)) = v(x) \\
&f_1(x) = af(x) + bg(x) \Longrightarrow df_1(x) = adf(x) + bdg(x)\\
&g_1(x) = cf(x) + dg(x) \Longrightarrow  bg_1(x) = bcf(x) + bdg(x)\\
&(ad-bc) f_1(x) = df_1(x) - bg_1(x) \\
&\qquad\Longrightarrow f(x) = \frac{d}{ad-bc}f_1(x) + \frac{b}{bc-ad}g_1(x)\\
&\mbox{同理} g(x) = \frac{a}{bc-ad}f_1(x) + \frac{c}{ad-bc}g_1(x)\\
\\
&\mbox{由前面的结论易知} v(x) | u(x)\\
&\Longrightarrow u(x) | v(x), v(x) | u(x), u(x) = v(x)\\
&\mbox{证毕}
\end{align*}

\end{document}